{
  "@id": "https://stencila.org/ArrayValidator",
  "name": "ArrayValidator",
  "license": "https://creativecommons.org/publicdomain/zero/1.0/",
  "@context": {
    "rdfs": "http://www.w3.org/2000/01/rdf-schema#",
    "schema": "https://schema.org/",
    "stencila": "https://stencila.org/"
  },
  "@graph": [
    {
      "@id": "stencila:ArrayValidator",
      "@type": "rdfs:Class",
      "rdfs:label": "ArrayValidator",
      "rdfs:comment": "A validator specifying constraints on an array node.",
      "rdfs:subClassOf": {
        "@id": "stencila:Entity"
      }
    },
    {
      "@id": "stencila:itemsNullable",
      "@type": "rdfs:Property",
      "rdfs:label": "itemsNullable",
      "rdfs:comment": "Whether items can have the value `Node::Null`",
      "schema:domainIncludes": {
        "@id": "stencila:ArrayValidator"
      },
      "schema:rangeIncludes": {
        "@id": "schema:Boolean"
      }
    },
    {
      "@id": "stencila:itemsValidator",
      "@type": "rdfs:Property",
      "rdfs:label": "itemsValidator",
      "rdfs:comment": "Another validator node specifying the constraints on all items in the array.",
      "schema:domainIncludes": {
        "@id": "stencila:ArrayValidator"
      },
      "schema:rangeIncludes": {
        "@id": "stencila:Validator"
      }
    },
    {
      "@id": "stencila:contains",
      "@type": "rdfs:Property",
      "rdfs:label": "contains",
      "rdfs:comment": "An array node is valid if at least one of its items is valid against the `contains` schema.",
      "schema:domainIncludes": {
        "@id": "stencila:ArrayValidator"
      },
      "schema:rangeIncludes": {
        "@id": "stencila:Validator"
      }
    },
    {
      "@id": "stencila:minItems",
      "@type": "rdfs:Property",
      "rdfs:label": "minItems",
      "rdfs:comment": "An array node is valid if its size is greater than, or equal to, this value.",
      "schema:domainIncludes": {
        "@id": "stencila:ArrayValidator"
      },
      "schema:rangeIncludes": {
        "@id": "schema:Number"
      }
    },
    {
      "@id": "stencila:maxItems",
      "@type": "rdfs:Property",
      "rdfs:label": "maxItems",
      "rdfs:comment": "An array node is valid if its size is less than, or equal to, this value.",
      "schema:domainIncludes": {
        "@id": "stencila:ArrayValidator"
      },
      "schema:rangeIncludes": {
        "@id": "schema:Number"
      }
    },
    {
      "@id": "stencila:uniqueItems",
      "@type": "rdfs:Property",
      "rdfs:label": "uniqueItems",
      "rdfs:comment": "A flag to indicate that each value in the array should be unique.",
      "schema:domainIncludes": {
        "@id": "stencila:ArrayValidator"
      },
      "schema:rangeIncludes": {
        "@id": "schema:Boolean"
      }
    }
  ]
}