{
  "@id": "https://stencila.dev/CompilationDigest",
  "name": "CompilationDigest",
  "license": "https://creativecommons.org/publicdomain/zero/1.0/",
  "@context": {
    "rdfs": "http://www.w3.org/2000/01/rdf-schema#",
    "schema": "https://schema.org/",
    "stencila": "https://stencila.dev/"
  },
  "@graph": [
    {
      "@id": "stencila:CompilationDigest",
      "@type": "rdfs:Class",
      "rdfs:label": "CompilationDigest",
      "rdfs:comment": "A digest of the content, semantics and dependencies of an executable node.",
      "rdfs:subClassOf": {
        "@id": "stencila:Entity"
      }
    },
    {
      "@id": "stencila:stateDigest",
      "@type": "rdfs:Property",
      "rdfs:label": "stateDigest",
      "rdfs:comment": "A digest of the state of a node.",
      "schema:domainIncludes": {
        "@id": "stencila:CompilationDigest"
      },
      "schema:rangeIncludes": {
        "@id": "stencila:UnsignedInteger"
      }
    },
    {
      "@id": "stencila:semanticDigest",
      "@type": "rdfs:Property",
      "rdfs:label": "semanticDigest",
      "rdfs:comment": "A digest of the semantics of the node with respect to the dependency graph.",
      "schema:domainIncludes": {
        "@id": "stencila:CompilationDigest"
      },
      "schema:rangeIncludes": {
        "@id": "stencila:UnsignedInteger"
      }
    },
    {
      "@id": "stencila:dependenciesDigest",
      "@type": "rdfs:Property",
      "rdfs:label": "dependenciesDigest",
      "rdfs:comment": "A digest of the semantic digests of the dependencies of a node.",
      "schema:domainIncludes": {
        "@id": "stencila:CompilationDigest"
      },
      "schema:rangeIncludes": {
        "@id": "stencila:UnsignedInteger"
      }
    },
    {
      "@id": "stencila:dependenciesStale",
      "@type": "rdfs:Property",
      "rdfs:label": "dependenciesStale",
      "rdfs:comment": "A count of the number of dependencies that are stale.",
      "schema:domainIncludes": {
        "@id": "stencila:CompilationDigest"
      },
      "schema:rangeIncludes": {
        "@id": "stencila:UnsignedInteger"
      }
    },
    {
      "@id": "stencila:dependenciesFailed",
      "@type": "rdfs:Property",
      "rdfs:label": "dependenciesFailed",
      "rdfs:comment": "A count of the number of dependencies that failed.",
      "schema:domainIncludes": {
        "@id": "stencila:CompilationDigest"
      },
      "schema:rangeIncludes": {
        "@id": "stencila:UnsignedInteger"
      }
    }
  ]
}